Get rid of all "class kinds" edits.

examples/shuffle/lib/Control/Monad/Random/Class.v
@@ -64,568 +64,606 @@ Import GHC.Base.Notations.
 
 (* Converted type declarations: *)
 
-Record MonadRandom__Dict m := MonadRandom__Dict_Build {
-  getRandom__ : forall {a}, forall `{(System.Random.Random a)}, m a ;
-  getRandomR__ : forall {a},
-  forall `{(System.Random.Random a)}, (a * a)%type -> m a ;
-  getRandomRs__ : forall {a},
-  forall `{(System.Random.Random a)}, (a * a)%type -> m (list a) ;
-  getRandoms__ : forall {a}, forall `{(System.Random.Random a)}, m (list a) }.
+Record MonadRandom__Dict (m : Type -> Type) := MonadRandom__Dict_Build {
+  getRandom__ : forall {a : Type}, forall `{System.Random.Random a}, m a ;
+  getRandomR__ : forall {a : Type},
+  forall `{System.Random.Random a}, (a * a)%type -> m a ;
+  getRandomRs__ : forall {a : Type},
+  forall `{System.Random.Random a}, (a * a)%type -> m (list a) ;
+  getRandoms__ : forall {a : Type},
+  forall `{System.Random.Random a}, m (list a) }.
 
-Definition MonadRandom m `{(GHC.Base.Monad m)} :=
+Definition MonadRandom (m : Type -> Type) `{GHC.Base.Monad m} :=
   forall r__, (MonadRandom__Dict m -> r__) -> r__.
-
 Existing Class MonadRandom.
 
+Record MonadInterleave__Dict (m : Type -> Type) := MonadInterleave__Dict_Build {
+  interleave__ : forall {a : Type}, m a -> m a }.
+
 Definition getRandom `{g__0__ : MonadRandom m}
-   : forall {a}, forall `{(System.Random.Random a)}, m a :=
+   : forall {a : Type}, forall `{System.Random.Random a}, m a :=
   g__0__ _ (getRandom__ m).
 
 Definition getRandomR `{g__0__ : MonadRandom m}
-   : forall {a}, forall `{(System.Random.Random a)}, (a * a)%type -> m a :=
+   : forall {a : Type}, forall `{System.Random.Random a}, (a * a)%type -> m a :=
   g__0__ _ (getRandomR__ m).
 
 Definition getRandomRs `{g__0__ : MonadRandom m}
-   : forall {a}, forall `{(System.Random.Random a)}, (a * a)%type -> m (list a) :=
+   : forall {a : Type},
+     forall `{System.Random.Random a}, (a * a)%type -> m (list a) :=
   g__0__ _ (getRandomRs__ m).
 
 Definition getRandoms `{g__0__ : MonadRandom m}
-   : forall {a}, forall `{(System.Random.Random a)}, m (list a) :=
+   : forall {a : Type}, forall `{System.Random.Random a}, m (list a) :=
   g__0__ _ (getRandoms__ m).
-
-Record MonadInterleave__Dict (m : Type -> Type) := MonadInterleave__Dict_Build {
-  interleave__ : forall {a}, m a -> m a }.
 
 Definition MonadInterleave (m : Type -> Type) `{MonadRandom m} :=
   forall r__, (MonadInterleave__Dict m -> r__) -> r__.
-
 Existing Class MonadInterleave.
 
-Definition interleave `{g__0__ : MonadInterleave m} : forall {a}, m a -> m a :=
+Definition interleave `{g__0__ : MonadInterleave m}
+   : forall {a : Type}, m a -> m a :=
   g__0__ _ (interleave__ m).
 
 (* Converted value declarations: *)
 
-(* Skipping instance `Control.Monad.Random.Class.MonadRandom__Strict_WriterT' of
-   class `Control.Monad.Random.Class.MonadRandom' *)
-
-Local Definition MonadRandom__WriterT_getRandom {inst_m} {inst_w} `{MonadRandom
-  inst_m} `{GHC.Base.Monoid inst_w}
-   : forall {a},
-     forall `{(System.Random.Random a)},
-     (Control.Monad.Trans.Writer.Lazy.WriterT inst_w inst_m) a :=
-  fun {a} `{(System.Random.Random a)} => Control.Monad.Trans.Class.lift getRandom.
-
-Local Definition MonadRandom__WriterT_getRandomR {inst_m} {inst_w} `{MonadRandom
-  inst_m} `{GHC.Base.Monoid inst_w}
-   : forall {a},
-     forall `{(System.Random.Random a)},
-     (a * a)%type -> (Control.Monad.Trans.Writer.Lazy.WriterT inst_w inst_m) a :=
-  fun {a} `{(System.Random.Random a)} =>
-    Control.Monad.Trans.Class.lift GHC.Base.∘ getRandomR.
-
-Local Definition MonadRandom__WriterT_getRandomRs {inst_m} {inst_w}
-  `{MonadRandom inst_m} `{GHC.Base.Monoid inst_w}
-   : forall {a},
-     forall `{(System.Random.Random a)},
-     (a * a)%type ->
-     (Control.Monad.Trans.Writer.Lazy.WriterT inst_w inst_m) (list a) :=
-  fun {a} `{(System.Random.Random a)} =>
-    Control.Monad.Trans.Class.lift GHC.Base.∘ getRandomRs.
-
-Local Definition MonadRandom__WriterT_getRandoms {inst_m} {inst_w} `{MonadRandom
-  inst_m} `{GHC.Base.Monoid inst_w}
-   : forall {a},
-     forall `{(System.Random.Random a)},
-     (Control.Monad.Trans.Writer.Lazy.WriterT inst_w inst_m) (list a) :=
-  fun {a} `{(System.Random.Random a)} =>
-    Control.Monad.Trans.Class.lift getRandoms.
-
-Program Instance MonadRandom__WriterT {m} {w} `{MonadRandom m} `{GHC.Base.Monoid
-  w}
-   : MonadRandom (Control.Monad.Trans.Writer.Lazy.WriterT w m) :=
-  fun _ k__ =>
-    k__ {| getRandom__ := fun {a} `{(System.Random.Random a)} =>
-             MonadRandom__WriterT_getRandom ;
-           getRandomR__ := fun {a} `{(System.Random.Random a)} =>
-             MonadRandom__WriterT_getRandomR ;
-           getRandomRs__ := fun {a} `{(System.Random.Random a)} =>
-             MonadRandom__WriterT_getRandomRs ;
-           getRandoms__ := fun {a} `{(System.Random.Random a)} =>
-             MonadRandom__WriterT_getRandoms |}.
-
-(* Skipping instance `Control.Monad.Random.Class.MonadRandom__Strict_StateT' of
-   class `Control.Monad.Random.Class.MonadRandom' *)
-
-Local Definition MonadRandom__StateT_getRandom {inst_m} {inst_s} `{(MonadRandom
-   inst_m)}
-   : forall {a},
-     forall `{(System.Random.Random a)},
-     (Control.Monad.Trans.State.Lazy.StateT inst_s inst_m) a :=
-  fun {a} `{(System.Random.Random a)} => Control.Monad.Trans.Class.lift getRandom.
-
-Local Definition MonadRandom__StateT_getRandomR {inst_m} {inst_s} `{(MonadRandom
-   inst_m)}
-   : forall {a},
-     forall `{(System.Random.Random a)},
-     (a * a)%type -> (Control.Monad.Trans.State.Lazy.StateT inst_s inst_m) a :=
-  fun {a} `{(System.Random.Random a)} =>
-    Control.Monad.Trans.Class.lift GHC.Base.∘ getRandomR.
-
-Local Definition MonadRandom__StateT_getRandomRs {inst_m} {inst_s}
-  `{(MonadRandom inst_m)}
-   : forall {a},
-     forall `{(System.Random.Random a)},
-     (a * a)%type ->
-     (Control.Monad.Trans.State.Lazy.StateT inst_s inst_m) (list a) :=
-  fun {a} `{(System.Random.Random a)} =>
-    Control.Monad.Trans.Class.lift GHC.Base.∘ getRandomRs.
-
-Local Definition MonadRandom__StateT_getRandoms {inst_m} {inst_s} `{(MonadRandom
-   inst_m)}
-   : forall {a},
-     forall `{(System.Random.Random a)},
-     (Control.Monad.Trans.State.Lazy.StateT inst_s inst_m) (list a) :=
-  fun {a} `{(System.Random.Random a)} =>
-    Control.Monad.Trans.Class.lift getRandoms.
-
-Program Instance MonadRandom__StateT {m} {s} `{(MonadRandom m)}
-   : MonadRandom (Control.Monad.Trans.State.Lazy.StateT s m) :=
-  fun _ k__ =>
-    k__ {| getRandom__ := fun {a} `{(System.Random.Random a)} =>
-             MonadRandom__StateT_getRandom ;
-           getRandomR__ := fun {a} `{(System.Random.Random a)} =>
-             MonadRandom__StateT_getRandomR ;
-           getRandomRs__ := fun {a} `{(System.Random.Random a)} =>
-             MonadRandom__StateT_getRandomRs ;
-           getRandoms__ := fun {a} `{(System.Random.Random a)} =>
-             MonadRandom__StateT_getRandoms |}.
-
-Local Definition MonadRandom__ReaderT_getRandom {inst_m} {inst_r} `{(MonadRandom
-   inst_m)}
-   : forall {a},
-     forall `{(System.Random.Random a)},
-     (Control.Monad.Trans.Reader.ReaderT inst_r inst_m) a :=
-  fun {a} `{(System.Random.Random a)} => Control.Monad.Trans.Class.lift getRandom.
-
-Local Definition MonadRandom__ReaderT_getRandomR {inst_m} {inst_r}
-  `{(MonadRandom inst_m)}
-   : forall {a},
-     forall `{(System.Random.Random a)},
-     (a * a)%type -> (Control.Monad.Trans.Reader.ReaderT inst_r inst_m) a :=
-  fun {a} `{(System.Random.Random a)} =>
-    Control.Monad.Trans.Class.lift GHC.Base.∘ getRandomR.
-
-Local Definition MonadRandom__ReaderT_getRandomRs {inst_m} {inst_r}
-  `{(MonadRandom inst_m)}
-   : forall {a},
-     forall `{(System.Random.Random a)},
-     (a * a)%type -> (Control.Monad.Trans.Reader.ReaderT inst_r inst_m) (list a) :=
-  fun {a} `{(System.Random.Random a)} =>
-    Control.Monad.Trans.Class.lift GHC.Base.∘ getRandomRs.
-
-Local Definition MonadRandom__ReaderT_getRandoms {inst_m} {inst_r}
-  `{(MonadRandom inst_m)}
-   : forall {a},
-     forall `{(System.Random.Random a)},
-     (Control.Monad.Trans.Reader.ReaderT inst_r inst_m) (list a) :=
-  fun {a} `{(System.Random.Random a)} =>
-    Control.Monad.Trans.Class.lift getRandoms.
-
-Program Instance MonadRandom__ReaderT {m} {r} `{(MonadRandom m)}
-   : MonadRandom (Control.Monad.Trans.Reader.ReaderT r m) :=
-  fun _ k__ =>
-    k__ {| getRandom__ := fun {a} `{(System.Random.Random a)} =>
-             MonadRandom__ReaderT_getRandom ;
-           getRandomR__ := fun {a} `{(System.Random.Random a)} =>
-             MonadRandom__ReaderT_getRandomR ;
-           getRandomRs__ := fun {a} `{(System.Random.Random a)} =>
-             MonadRandom__ReaderT_getRandomRs ;
-           getRandoms__ := fun {a} `{(System.Random.Random a)} =>
-             MonadRandom__ReaderT_getRandoms |}.
-
-(* Skipping instance `Control.Monad.Random.Class.MonadRandom__Strict_RWST' of
-   class `Control.Monad.Random.Class.MonadRandom' *)
-
-Local Definition MonadRandom__RWST_getRandom {inst_w} {inst_m} {inst_r} {inst_s}
-  `{GHC.Base.Monoid inst_w} `{MonadRandom inst_m}
-   : forall {a},
-     forall `{(System.Random.Random a)},
-     (Control.Monad.Trans.RWS.Lazy.RWST inst_r inst_w inst_s inst_m) a :=
-  fun {a} `{(System.Random.Random a)} => Control.Monad.Trans.Class.lift getRandom.
-
-Local Definition MonadRandom__RWST_getRandomR {inst_w} {inst_m} {inst_r}
-  {inst_s} `{GHC.Base.Monoid inst_w} `{MonadRandom inst_m}
-   : forall {a},
-     forall `{(System.Random.Random a)},
-     (a * a)%type ->
-     (Control.Monad.Trans.RWS.Lazy.RWST inst_r inst_w inst_s inst_m) a :=
-  fun {a} `{(System.Random.Random a)} =>
-    Control.Monad.Trans.Class.lift GHC.Base.∘ getRandomR.
-
-Local Definition MonadRandom__RWST_getRandomRs {inst_w} {inst_m} {inst_r}
-  {inst_s} `{GHC.Base.Monoid inst_w} `{MonadRandom inst_m}
-   : forall {a},
-     forall `{(System.Random.Random a)},
-     (a * a)%type ->
-     (Control.Monad.Trans.RWS.Lazy.RWST inst_r inst_w inst_s inst_m) (list a) :=
-  fun {a} `{(System.Random.Random a)} =>
-    Control.Monad.Trans.Class.lift GHC.Base.∘ getRandomRs.
-
-Local Definition MonadRandom__RWST_getRandoms {inst_w} {inst_m} {inst_r}
-  {inst_s} `{GHC.Base.Monoid inst_w} `{MonadRandom inst_m}
-   : forall {a},
-     forall `{(System.Random.Random a)},
-     (Control.Monad.Trans.RWS.Lazy.RWST inst_r inst_w inst_s inst_m) (list a) :=
-  fun {a} `{(System.Random.Random a)} =>
-    Control.Monad.Trans.Class.lift getRandoms.
-
-Program Instance MonadRandom__RWST {w} {m} {r} {s} `{GHC.Base.Monoid w}
-  `{MonadRandom m}
-   : MonadRandom (Control.Monad.Trans.RWS.Lazy.RWST r w s m) :=
-  fun _ k__ =>
-    k__ {| getRandom__ := fun {a} `{(System.Random.Random a)} =>
-             MonadRandom__RWST_getRandom ;
-           getRandomR__ := fun {a} `{(System.Random.Random a)} =>
-             MonadRandom__RWST_getRandomR ;
-           getRandomRs__ := fun {a} `{(System.Random.Random a)} =>
-             MonadRandom__RWST_getRandomRs ;
-           getRandoms__ := fun {a} `{(System.Random.Random a)} =>
-             MonadRandom__RWST_getRandoms |}.
-
-Local Definition MonadRandom__MaybeT_getRandom {inst_m} `{(MonadRandom inst_m)}
-   : forall {a},
-     forall `{(System.Random.Random a)},
-     (Control.Monad.Trans.Maybe.MaybeT inst_m) a :=
-  fun {a} `{(System.Random.Random a)} => Control.Monad.Trans.Class.lift getRandom.
-
-Local Definition MonadRandom__MaybeT_getRandomR {inst_m} `{(MonadRandom inst_m)}
-   : forall {a},
-     forall `{(System.Random.Random a)},
-     (a * a)%type -> (Control.Monad.Trans.Maybe.MaybeT inst_m) a :=
-  fun {a} `{(System.Random.Random a)} =>
-    Control.Monad.Trans.Class.lift GHC.Base.∘ getRandomR.
-
-Local Definition MonadRandom__MaybeT_getRandomRs {inst_m} `{(MonadRandom
-   inst_m)}
-   : forall {a},
-     forall `{(System.Random.Random a)},
-     (a * a)%type -> (Control.Monad.Trans.Maybe.MaybeT inst_m) (list a) :=
-  fun {a} `{(System.Random.Random a)} =>
-    Control.Monad.Trans.Class.lift GHC.Base.∘ getRandomRs.
-
-Local Definition MonadRandom__MaybeT_getRandoms {inst_m} `{(MonadRandom inst_m)}
-   : forall {a},
-     forall `{(System.Random.Random a)},
-     (Control.Monad.Trans.Maybe.MaybeT inst_m) (list a) :=
-  fun {a} `{(System.Random.Random a)} =>
-    Control.Monad.Trans.Class.lift getRandoms.
-
-Program Instance MonadRandom__MaybeT {m} `{(MonadRandom m)}
-   : MonadRandom (Control.Monad.Trans.Maybe.MaybeT m) :=
-  fun _ k__ =>
-    k__ {| getRandom__ := fun {a} `{(System.Random.Random a)} =>
-             MonadRandom__MaybeT_getRandom ;
-           getRandomR__ := fun {a} `{(System.Random.Random a)} =>
-             MonadRandom__MaybeT_getRandomR ;
-           getRandomRs__ := fun {a} `{(System.Random.Random a)} =>
-             MonadRandom__MaybeT_getRandomRs ;
-           getRandoms__ := fun {a} `{(System.Random.Random a)} =>
-             MonadRandom__MaybeT_getRandoms |}.
-
-(* Skipping instance `Control.Monad.Random.Class.MonadRandom__ListT' of class
+(* Skipping instance `Control.Monad.Random.Class.MonadRandom__IO' of class
    `Control.Monad.Random.Class.MonadRandom' *)
 
-Local Definition MonadRandom__IdentityT_getRandom {inst_m} `{(MonadRandom
-   inst_m)}
-   : forall {a},
-     forall `{(System.Random.Random a)},
-     (Control.Monad.Trans.Identity.IdentityT inst_m) a :=
-  fun {a} `{(System.Random.Random a)} => Control.Monad.Trans.Class.lift getRandom.
+Local Definition MonadRandom__ContT_getRandom {inst_m : Type -> Type} {inst_r
+   : Type} `{(MonadRandom inst_m)}
+   : forall {a : Type},
+     forall `{System.Random.Random a},
+     Control.Monad.Trans.Cont.ContT inst_r inst_m a :=
+  fun {a : Type} `{System.Random.Random a} =>
+    Control.Monad.Trans.Class.lift getRandom.
 
-Local Definition MonadRandom__IdentityT_getRandomR {inst_m} `{(MonadRandom
-   inst_m)}
-   : forall {a},
-     forall `{(System.Random.Random a)},
-     (a * a)%type -> (Control.Monad.Trans.Identity.IdentityT inst_m) a :=
-  fun {a} `{(System.Random.Random a)} =>
+Local Definition MonadRandom__ContT_getRandomR {inst_m : Type -> Type} {inst_r
+   : Type} `{(MonadRandom inst_m)}
+   : forall {a : Type},
+     forall `{System.Random.Random a},
+     (a * a)%type -> Control.Monad.Trans.Cont.ContT inst_r inst_m a :=
+  fun {a : Type} `{System.Random.Random a} =>
     Control.Monad.Trans.Class.lift GHC.Base.∘ getRandomR.
 
-Local Definition MonadRandom__IdentityT_getRandomRs {inst_m} `{(MonadRandom
-   inst_m)}
-   : forall {a},
-     forall `{(System.Random.Random a)},
-     (a * a)%type -> (Control.Monad.Trans.Identity.IdentityT inst_m) (list a) :=
-  fun {a} `{(System.Random.Random a)} =>
+Local Definition MonadRandom__ContT_getRandomRs {inst_m : Type -> Type} {inst_r
+   : Type} `{(MonadRandom inst_m)}
+   : forall {a : Type},
+     forall `{System.Random.Random a},
+     (a * a)%type -> Control.Monad.Trans.Cont.ContT inst_r inst_m (list a) :=
+  fun {a : Type} `{System.Random.Random a} =>
     Control.Monad.Trans.Class.lift GHC.Base.∘ getRandomRs.
 
-Local Definition MonadRandom__IdentityT_getRandoms {inst_m} `{(MonadRandom
-   inst_m)}
-   : forall {a},
-     forall `{(System.Random.Random a)},
-     (Control.Monad.Trans.Identity.IdentityT inst_m) (list a) :=
-  fun {a} `{(System.Random.Random a)} =>
+Local Definition MonadRandom__ContT_getRandoms {inst_m : Type -> Type} {inst_r
+   : Type} `{(MonadRandom inst_m)}
+   : forall {a : Type},
+     forall `{System.Random.Random a},
+     Control.Monad.Trans.Cont.ContT inst_r inst_m (list a) :=
+  fun {a : Type} `{System.Random.Random a} =>
     Control.Monad.Trans.Class.lift getRandoms.
 
-Program Instance MonadRandom__IdentityT {m} `{(MonadRandom m)}
-   : MonadRandom (Control.Monad.Trans.Identity.IdentityT m) :=
+Program Instance MonadRandom__ContT {m : Type -> Type} {r : Type} `{(MonadRandom
+   m)}
+   : MonadRandom (Control.Monad.Trans.Cont.ContT r m) :=
   fun _ k__ =>
-    k__ {| getRandom__ := fun {a} `{(System.Random.Random a)} =>
-             MonadRandom__IdentityT_getRandom ;
-           getRandomR__ := fun {a} `{(System.Random.Random a)} =>
-             MonadRandom__IdentityT_getRandomR ;
-           getRandomRs__ := fun {a} `{(System.Random.Random a)} =>
-             MonadRandom__IdentityT_getRandomRs ;
-           getRandoms__ := fun {a} `{(System.Random.Random a)} =>
-             MonadRandom__IdentityT_getRandoms |}.
-
-Local Definition MonadRandom__ExceptT_getRandom {inst_m} {inst_e} `{(MonadRandom
-   inst_m)}
-   : forall {a},
-     forall `{(System.Random.Random a)},
-     (Control.Monad.Trans.Except.ExceptT inst_e inst_m) a :=
-  fun {a} `{(System.Random.Random a)} => Control.Monad.Trans.Class.lift getRandom.
-
-Local Definition MonadRandom__ExceptT_getRandomR {inst_m} {inst_e}
-  `{(MonadRandom inst_m)}
-   : forall {a},
-     forall `{(System.Random.Random a)},
-     (a * a)%type -> (Control.Monad.Trans.Except.ExceptT inst_e inst_m) a :=
-  fun {a} `{(System.Random.Random a)} =>
-    Control.Monad.Trans.Class.lift GHC.Base.∘ getRandomR.
-
-Local Definition MonadRandom__ExceptT_getRandomRs {inst_m} {inst_e}
-  `{(MonadRandom inst_m)}
-   : forall {a},
-     forall `{(System.Random.Random a)},
-     (a * a)%type -> (Control.Monad.Trans.Except.ExceptT inst_e inst_m) (list a) :=
-  fun {a} `{(System.Random.Random a)} =>
-    Control.Monad.Trans.Class.lift GHC.Base.∘ getRandomRs.
-
-Local Definition MonadRandom__ExceptT_getRandoms {inst_m} {inst_e}
-  `{(MonadRandom inst_m)}
-   : forall {a},
-     forall `{(System.Random.Random a)},
-     (Control.Monad.Trans.Except.ExceptT inst_e inst_m) (list a) :=
-  fun {a} `{(System.Random.Random a)} =>
-    Control.Monad.Trans.Class.lift getRandoms.
-
-Program Instance MonadRandom__ExceptT {m} {e} `{(MonadRandom m)}
-   : MonadRandom (Control.Monad.Trans.Except.ExceptT e m) :=
-  fun _ k__ =>
-    k__ {| getRandom__ := fun {a} `{(System.Random.Random a)} =>
-             MonadRandom__ExceptT_getRandom ;
-           getRandomR__ := fun {a} `{(System.Random.Random a)} =>
-             MonadRandom__ExceptT_getRandomR ;
-           getRandomRs__ := fun {a} `{(System.Random.Random a)} =>
-             MonadRandom__ExceptT_getRandomRs ;
-           getRandoms__ := fun {a} `{(System.Random.Random a)} =>
-             MonadRandom__ExceptT_getRandoms |}.
+    k__ {| getRandom__ := fun {a : Type} `{System.Random.Random a} =>
+             MonadRandom__ContT_getRandom ;
+           getRandomR__ := fun {a : Type} `{System.Random.Random a} =>
+             MonadRandom__ContT_getRandomR ;
+           getRandomRs__ := fun {a : Type} `{System.Random.Random a} =>
+             MonadRandom__ContT_getRandomRs ;
+           getRandoms__ := fun {a : Type} `{System.Random.Random a} =>
+             MonadRandom__ContT_getRandoms |}.
 
 (* Skipping instance `Control.Monad.Random.Class.MonadRandom__ErrorT' of class
    `Control.Monad.Random.Class.MonadRandom' *)
 
-Local Definition MonadRandom__ContT_getRandom {inst_m} {inst_r} `{(MonadRandom
-   inst_m)}
-   : forall {a},
-     forall `{(System.Random.Random a)},
-     (Control.Monad.Trans.Cont.ContT inst_r inst_m) a :=
-  fun {a} `{(System.Random.Random a)} => Control.Monad.Trans.Class.lift getRandom.
+Local Definition MonadRandom__ExceptT_getRandom {inst_m : Type -> Type} {inst_e
+   : Type} `{(MonadRandom inst_m)}
+   : forall {a : Type},
+     forall `{System.Random.Random a},
+     Control.Monad.Trans.Except.ExceptT inst_e inst_m a :=
+  fun {a : Type} `{System.Random.Random a} =>
+    Control.Monad.Trans.Class.lift getRandom.
 
-Local Definition MonadRandom__ContT_getRandomR {inst_m} {inst_r} `{(MonadRandom
-   inst_m)}
-   : forall {a},
-     forall `{(System.Random.Random a)},
-     (a * a)%type -> (Control.Monad.Trans.Cont.ContT inst_r inst_m) a :=
-  fun {a} `{(System.Random.Random a)} =>
+Local Definition MonadRandom__ExceptT_getRandomR {inst_m : Type -> Type} {inst_e
+   : Type} `{(MonadRandom inst_m)}
+   : forall {a : Type},
+     forall `{System.Random.Random a},
+     (a * a)%type -> Control.Monad.Trans.Except.ExceptT inst_e inst_m a :=
+  fun {a : Type} `{System.Random.Random a} =>
     Control.Monad.Trans.Class.lift GHC.Base.∘ getRandomR.
 
-Local Definition MonadRandom__ContT_getRandomRs {inst_m} {inst_r} `{(MonadRandom
-   inst_m)}
-   : forall {a},
-     forall `{(System.Random.Random a)},
-     (a * a)%type -> (Control.Monad.Trans.Cont.ContT inst_r inst_m) (list a) :=
-  fun {a} `{(System.Random.Random a)} =>
+Local Definition MonadRandom__ExceptT_getRandomRs {inst_m : Type -> Type}
+  {inst_e : Type} `{(MonadRandom inst_m)}
+   : forall {a : Type},
+     forall `{System.Random.Random a},
+     (a * a)%type -> Control.Monad.Trans.Except.ExceptT inst_e inst_m (list a) :=
+  fun {a : Type} `{System.Random.Random a} =>
     Control.Monad.Trans.Class.lift GHC.Base.∘ getRandomRs.
 
-Local Definition MonadRandom__ContT_getRandoms {inst_m} {inst_r} `{(MonadRandom
-   inst_m)}
-   : forall {a},
-     forall `{(System.Random.Random a)},
-     (Control.Monad.Trans.Cont.ContT inst_r inst_m) (list a) :=
-  fun {a} `{(System.Random.Random a)} =>
+Local Definition MonadRandom__ExceptT_getRandoms {inst_m : Type -> Type} {inst_e
+   : Type} `{(MonadRandom inst_m)}
+   : forall {a : Type},
+     forall `{System.Random.Random a},
+     Control.Monad.Trans.Except.ExceptT inst_e inst_m (list a) :=
+  fun {a : Type} `{System.Random.Random a} =>
     Control.Monad.Trans.Class.lift getRandoms.
 
-Program Instance MonadRandom__ContT {m} {r} `{(MonadRandom m)}
-   : MonadRandom (Control.Monad.Trans.Cont.ContT r m) :=
+Program Instance MonadRandom__ExceptT {m : Type -> Type} {e : Type}
+  `{(MonadRandom m)}
+   : MonadRandom (Control.Monad.Trans.Except.ExceptT e m) :=
   fun _ k__ =>
-    k__ {| getRandom__ := fun {a} `{(System.Random.Random a)} =>
-             MonadRandom__ContT_getRandom ;
-           getRandomR__ := fun {a} `{(System.Random.Random a)} =>
-             MonadRandom__ContT_getRandomR ;
-           getRandomRs__ := fun {a} `{(System.Random.Random a)} =>
-             MonadRandom__ContT_getRandomRs ;
-           getRandoms__ := fun {a} `{(System.Random.Random a)} =>
-             MonadRandom__ContT_getRandoms |}.
+    k__ {| getRandom__ := fun {a : Type} `{System.Random.Random a} =>
+             MonadRandom__ExceptT_getRandom ;
+           getRandomR__ := fun {a : Type} `{System.Random.Random a} =>
+             MonadRandom__ExceptT_getRandomR ;
+           getRandomRs__ := fun {a : Type} `{System.Random.Random a} =>
+             MonadRandom__ExceptT_getRandomRs ;
+           getRandoms__ := fun {a : Type} `{System.Random.Random a} =>
+             MonadRandom__ExceptT_getRandoms |}.
 
-(* Skipping instance `Control.Monad.Random.Class.MonadRandom__IO' of class
+Local Definition MonadRandom__IdentityT_getRandom {inst_m : Type -> Type}
+  `{(MonadRandom inst_m)}
+   : forall {a : Type},
+     forall `{System.Random.Random a},
+     Control.Monad.Trans.Identity.IdentityT inst_m a :=
+  fun {a : Type} `{System.Random.Random a} =>
+    Control.Monad.Trans.Class.lift getRandom.
+
+Local Definition MonadRandom__IdentityT_getRandomR {inst_m : Type -> Type}
+  `{(MonadRandom inst_m)}
+   : forall {a : Type},
+     forall `{System.Random.Random a},
+     (a * a)%type -> Control.Monad.Trans.Identity.IdentityT inst_m a :=
+  fun {a : Type} `{System.Random.Random a} =>
+    Control.Monad.Trans.Class.lift GHC.Base.∘ getRandomR.
+
+Local Definition MonadRandom__IdentityT_getRandomRs {inst_m : Type -> Type}
+  `{(MonadRandom inst_m)}
+   : forall {a : Type},
+     forall `{System.Random.Random a},
+     (a * a)%type -> Control.Monad.Trans.Identity.IdentityT inst_m (list a) :=
+  fun {a : Type} `{System.Random.Random a} =>
+    Control.Monad.Trans.Class.lift GHC.Base.∘ getRandomRs.
+
+Local Definition MonadRandom__IdentityT_getRandoms {inst_m : Type -> Type}
+  `{(MonadRandom inst_m)}
+   : forall {a : Type},
+     forall `{System.Random.Random a},
+     Control.Monad.Trans.Identity.IdentityT inst_m (list a) :=
+  fun {a : Type} `{System.Random.Random a} =>
+    Control.Monad.Trans.Class.lift getRandoms.
+
+Program Instance MonadRandom__IdentityT {m : Type -> Type} `{(MonadRandom m)}
+   : MonadRandom (Control.Monad.Trans.Identity.IdentityT m) :=
+  fun _ k__ =>
+    k__ {| getRandom__ := fun {a : Type} `{System.Random.Random a} =>
+             MonadRandom__IdentityT_getRandom ;
+           getRandomR__ := fun {a : Type} `{System.Random.Random a} =>
+             MonadRandom__IdentityT_getRandomR ;
+           getRandomRs__ := fun {a : Type} `{System.Random.Random a} =>
+             MonadRandom__IdentityT_getRandomRs ;
+           getRandoms__ := fun {a : Type} `{System.Random.Random a} =>
+             MonadRandom__IdentityT_getRandoms |}.
+
+(* Skipping instance `Control.Monad.Random.Class.MonadRandom__ListT' of class
    `Control.Monad.Random.Class.MonadRandom' *)
 
-(* Skipping all instances of class `Control.Monad.Random.Class.MonadSplit',
-   including `Control.Monad.Random.Class.MonadSplit__Strict_WriterT__5' *)
+Local Definition MonadRandom__MaybeT_getRandom {inst_m : Type -> Type}
+  `{(MonadRandom inst_m)}
+   : forall {a : Type},
+     forall `{System.Random.Random a}, Control.Monad.Trans.Maybe.MaybeT inst_m a :=
+  fun {a : Type} `{System.Random.Random a} =>
+    Control.Monad.Trans.Class.lift getRandom.
+
+Local Definition MonadRandom__MaybeT_getRandomR {inst_m : Type -> Type}
+  `{(MonadRandom inst_m)}
+   : forall {a : Type},
+     forall `{System.Random.Random a},
+     (a * a)%type -> Control.Monad.Trans.Maybe.MaybeT inst_m a :=
+  fun {a : Type} `{System.Random.Random a} =>
+    Control.Monad.Trans.Class.lift GHC.Base.∘ getRandomR.
+
+Local Definition MonadRandom__MaybeT_getRandomRs {inst_m : Type -> Type}
+  `{(MonadRandom inst_m)}
+   : forall {a : Type},
+     forall `{System.Random.Random a},
+     (a * a)%type -> Control.Monad.Trans.Maybe.MaybeT inst_m (list a) :=
+  fun {a : Type} `{System.Random.Random a} =>
+    Control.Monad.Trans.Class.lift GHC.Base.∘ getRandomRs.
+
+Local Definition MonadRandom__MaybeT_getRandoms {inst_m : Type -> Type}
+  `{(MonadRandom inst_m)}
+   : forall {a : Type},
+     forall `{System.Random.Random a},
+     Control.Monad.Trans.Maybe.MaybeT inst_m (list a) :=
+  fun {a : Type} `{System.Random.Random a} =>
+    Control.Monad.Trans.Class.lift getRandoms.
+
+Program Instance MonadRandom__MaybeT {m : Type -> Type} `{(MonadRandom m)}
+   : MonadRandom (Control.Monad.Trans.Maybe.MaybeT m) :=
+  fun _ k__ =>
+    k__ {| getRandom__ := fun {a : Type} `{System.Random.Random a} =>
+             MonadRandom__MaybeT_getRandom ;
+           getRandomR__ := fun {a : Type} `{System.Random.Random a} =>
+             MonadRandom__MaybeT_getRandomR ;
+           getRandomRs__ := fun {a : Type} `{System.Random.Random a} =>
+             MonadRandom__MaybeT_getRandomRs ;
+           getRandoms__ := fun {a : Type} `{System.Random.Random a} =>
+             MonadRandom__MaybeT_getRandoms |}.
+
+Local Definition MonadRandom__RWST_getRandom {inst_w : Type} {inst_m
+   : Type -> Type} {inst_r : Type} {inst_s : Type} `{GHC.Base.Monoid inst_w}
+  `{MonadRandom inst_m}
+   : forall {a : Type},
+     forall `{System.Random.Random a},
+     Control.Monad.Trans.RWS.Lazy.RWST inst_r inst_w inst_s inst_m a :=
+  fun {a : Type} `{System.Random.Random a} =>
+    Control.Monad.Trans.Class.lift getRandom.
+
+Local Definition MonadRandom__RWST_getRandomR {inst_w : Type} {inst_m
+   : Type -> Type} {inst_r : Type} {inst_s : Type} `{GHC.Base.Monoid inst_w}
+  `{MonadRandom inst_m}
+   : forall {a : Type},
+     forall `{System.Random.Random a},
+     (a * a)%type ->
+     Control.Monad.Trans.RWS.Lazy.RWST inst_r inst_w inst_s inst_m a :=
+  fun {a : Type} `{System.Random.Random a} =>
+    Control.Monad.Trans.Class.lift GHC.Base.∘ getRandomR.
+
+Local Definition MonadRandom__RWST_getRandomRs {inst_w : Type} {inst_m
+   : Type -> Type} {inst_r : Type} {inst_s : Type} `{GHC.Base.Monoid inst_w}
+  `{MonadRandom inst_m}
+   : forall {a : Type},
+     forall `{System.Random.Random a},
+     (a * a)%type ->
+     Control.Monad.Trans.RWS.Lazy.RWST inst_r inst_w inst_s inst_m (list a) :=
+  fun {a : Type} `{System.Random.Random a} =>
+    Control.Monad.Trans.Class.lift GHC.Base.∘ getRandomRs.
+
+Local Definition MonadRandom__RWST_getRandoms {inst_w : Type} {inst_m
+   : Type -> Type} {inst_r : Type} {inst_s : Type} `{GHC.Base.Monoid inst_w}
+  `{MonadRandom inst_m}
+   : forall {a : Type},
+     forall `{System.Random.Random a},
+     Control.Monad.Trans.RWS.Lazy.RWST inst_r inst_w inst_s inst_m (list a) :=
+  fun {a : Type} `{System.Random.Random a} =>
+    Control.Monad.Trans.Class.lift getRandoms.
+
+Program Instance MonadRandom__RWST {w : Type} {m : Type -> Type} {r : Type} {s
+   : Type} `{GHC.Base.Monoid w} `{MonadRandom m}
+   : MonadRandom (Control.Monad.Trans.RWS.Lazy.RWST r w s m) :=
+  fun _ k__ =>
+    k__ {| getRandom__ := fun {a : Type} `{System.Random.Random a} =>
+             MonadRandom__RWST_getRandom ;
+           getRandomR__ := fun {a : Type} `{System.Random.Random a} =>
+             MonadRandom__RWST_getRandomR ;
+           getRandomRs__ := fun {a : Type} `{System.Random.Random a} =>
+             MonadRandom__RWST_getRandomRs ;
+           getRandoms__ := fun {a : Type} `{System.Random.Random a} =>
+             MonadRandom__RWST_getRandoms |}.
+
+(* Skipping instance `Control.Monad.Random.Class.MonadRandom__Strict_RWST' of
+   class `Control.Monad.Random.Class.MonadRandom' *)
+
+Local Definition MonadRandom__ReaderT_getRandom {inst_m : Type -> Type} {inst_r
+   : Type} `{(MonadRandom inst_m)}
+   : forall {a : Type},
+     forall `{System.Random.Random a},
+     Control.Monad.Trans.Reader.ReaderT inst_r inst_m a :=
+  fun {a : Type} `{System.Random.Random a} =>
+    Control.Monad.Trans.Class.lift getRandom.
+
+Local Definition MonadRandom__ReaderT_getRandomR {inst_m : Type -> Type} {inst_r
+   : Type} `{(MonadRandom inst_m)}
+   : forall {a : Type},
+     forall `{System.Random.Random a},
+     (a * a)%type -> Control.Monad.Trans.Reader.ReaderT inst_r inst_m a :=
+  fun {a : Type} `{System.Random.Random a} =>
+    Control.Monad.Trans.Class.lift GHC.Base.∘ getRandomR.
+
+Local Definition MonadRandom__ReaderT_getRandomRs {inst_m : Type -> Type}
+  {inst_r : Type} `{(MonadRandom inst_m)}
+   : forall {a : Type},
+     forall `{System.Random.Random a},
+     (a * a)%type -> Control.Monad.Trans.Reader.ReaderT inst_r inst_m (list a) :=
+  fun {a : Type} `{System.Random.Random a} =>
+    Control.Monad.Trans.Class.lift GHC.Base.∘ getRandomRs.
+
+Local Definition MonadRandom__ReaderT_getRandoms {inst_m : Type -> Type} {inst_r
+   : Type} `{(MonadRandom inst_m)}
+   : forall {a : Type},
+     forall `{System.Random.Random a},
+     Control.Monad.Trans.Reader.ReaderT inst_r inst_m (list a) :=
+  fun {a : Type} `{System.Random.Random a} =>
+    Control.Monad.Trans.Class.lift getRandoms.
+
+Program Instance MonadRandom__ReaderT {m : Type -> Type} {r : Type}
+  `{(MonadRandom m)}
+   : MonadRandom (Control.Monad.Trans.Reader.ReaderT r m) :=
+  fun _ k__ =>
+    k__ {| getRandom__ := fun {a : Type} `{System.Random.Random a} =>
+             MonadRandom__ReaderT_getRandom ;
+           getRandomR__ := fun {a : Type} `{System.Random.Random a} =>
+             MonadRandom__ReaderT_getRandomR ;
+           getRandomRs__ := fun {a : Type} `{System.Random.Random a} =>
+             MonadRandom__ReaderT_getRandomRs ;
+           getRandoms__ := fun {a : Type} `{System.Random.Random a} =>
+             MonadRandom__ReaderT_getRandoms |}.
+
+Local Definition MonadRandom__StateT_getRandom {inst_m : Type -> Type} {inst_s
+   : Type} `{(MonadRandom inst_m)}
+   : forall {a : Type},
+     forall `{System.Random.Random a},
+     Control.Monad.Trans.State.Lazy.StateT inst_s inst_m a :=
+  fun {a : Type} `{System.Random.Random a} =>
+    Control.Monad.Trans.Class.lift getRandom.
+
+Local Definition MonadRandom__StateT_getRandomR {inst_m : Type -> Type} {inst_s
+   : Type} `{(MonadRandom inst_m)}
+   : forall {a : Type},
+     forall `{System.Random.Random a},
+     (a * a)%type -> Control.Monad.Trans.State.Lazy.StateT inst_s inst_m a :=
+  fun {a : Type} `{System.Random.Random a} =>
+    Control.Monad.Trans.Class.lift GHC.Base.∘ getRandomR.
+
+Local Definition MonadRandom__StateT_getRandomRs {inst_m : Type -> Type} {inst_s
+   : Type} `{(MonadRandom inst_m)}
+   : forall {a : Type},
+     forall `{System.Random.Random a},
+     (a * a)%type -> Control.Monad.Trans.State.Lazy.StateT inst_s inst_m (list a) :=
+  fun {a : Type} `{System.Random.Random a} =>
+    Control.Monad.Trans.Class.lift GHC.Base.∘ getRandomRs.
+
+Local Definition MonadRandom__StateT_getRandoms {inst_m : Type -> Type} {inst_s
+   : Type} `{(MonadRandom inst_m)}
+   : forall {a : Type},
+     forall `{System.Random.Random a},
+     Control.Monad.Trans.State.Lazy.StateT inst_s inst_m (list a) :=
+  fun {a : Type} `{System.Random.Random a} =>
+    Control.Monad.Trans.Class.lift getRandoms.
+
+Program Instance MonadRandom__StateT {m : Type -> Type} {s : Type}
+  `{(MonadRandom m)}
+   : MonadRandom (Control.Monad.Trans.State.Lazy.StateT s m) :=
+  fun _ k__ =>
+    k__ {| getRandom__ := fun {a : Type} `{System.Random.Random a} =>
+             MonadRandom__StateT_getRandom ;
+           getRandomR__ := fun {a : Type} `{System.Random.Random a} =>
+             MonadRandom__StateT_getRandomR ;
+           getRandomRs__ := fun {a : Type} `{System.Random.Random a} =>
+             MonadRandom__StateT_getRandomRs ;
+           getRandoms__ := fun {a : Type} `{System.Random.Random a} =>
+             MonadRandom__StateT_getRandoms |}.
+
+(* Skipping instance `Control.Monad.Random.Class.MonadRandom__Strict_StateT' of
+   class `Control.Monad.Random.Class.MonadRandom' *)
+
+Local Definition MonadRandom__WriterT_getRandom {inst_m : Type -> Type} {inst_w
+   : Type} `{MonadRandom inst_m} `{GHC.Base.Monoid inst_w}
+   : forall {a : Type},
+     forall `{System.Random.Random a},
+     Control.Monad.Trans.Writer.Lazy.WriterT inst_w inst_m a :=
+  fun {a : Type} `{System.Random.Random a} =>
+    Control.Monad.Trans.Class.lift getRandom.
+
+Local Definition MonadRandom__WriterT_getRandomR {inst_m : Type -> Type} {inst_w
+   : Type} `{MonadRandom inst_m} `{GHC.Base.Monoid inst_w}
+   : forall {a : Type},
+     forall `{System.Random.Random a},
+     (a * a)%type -> Control.Monad.Trans.Writer.Lazy.WriterT inst_w inst_m a :=
+  fun {a : Type} `{System.Random.Random a} =>
+    Control.Monad.Trans.Class.lift GHC.Base.∘ getRandomR.
+
+Local Definition MonadRandom__WriterT_getRandomRs {inst_m : Type -> Type}
+  {inst_w : Type} `{MonadRandom inst_m} `{GHC.Base.Monoid inst_w}
+   : forall {a : Type},
+     forall `{System.Random.Random a},
+     (a * a)%type ->
+     Control.Monad.Trans.Writer.Lazy.WriterT inst_w inst_m (list a) :=
+  fun {a : Type} `{System.Random.Random a} =>
+    Control.Monad.Trans.Class.lift GHC.Base.∘ getRandomRs.
+
+Local Definition MonadRandom__WriterT_getRandoms {inst_m : Type -> Type} {inst_w
+   : Type} `{MonadRandom inst_m} `{GHC.Base.Monoid inst_w}
+   : forall {a : Type},
+     forall `{System.Random.Random a},
+     Control.Monad.Trans.Writer.Lazy.WriterT inst_w inst_m (list a) :=
+  fun {a : Type} `{System.Random.Random a} =>
+    Control.Monad.Trans.Class.lift getRandoms.
+
+Program Instance MonadRandom__WriterT {m : Type -> Type} {w : Type}
+  `{MonadRandom m} `{GHC.Base.Monoid w}
+   : MonadRandom (Control.Monad.Trans.Writer.Lazy.WriterT w m) :=
+  fun _ k__ =>
+    k__ {| getRandom__ := fun {a : Type} `{System.Random.Random a} =>
+             MonadRandom__WriterT_getRandom ;
+           getRandomR__ := fun {a : Type} `{System.Random.Random a} =>
+             MonadRandom__WriterT_getRandomR ;
+           getRandomRs__ := fun {a : Type} `{System.Random.Random a} =>
+             MonadRandom__WriterT_getRandomRs ;
+           getRandoms__ := fun {a : Type} `{System.Random.Random a} =>
+             MonadRandom__WriterT_getRandoms |}.
+
+(* Skipping instance `Control.Monad.Random.Class.MonadRandom__Strict_WriterT' of
+   class `Control.Monad.Random.Class.MonadRandom' *)
 
 (* Skipping all instances of class `Control.Monad.Random.Class.MonadSplit',
-   including `Control.Monad.Random.Class.MonadSplit__WriterT__5' *)
-
-(* Skipping all instances of class `Control.Monad.Random.Class.MonadSplit',
-   including `Control.Monad.Random.Class.MonadSplit__Strict_StateT__5' *)
-
-(* Skipping all instances of class `Control.Monad.Random.Class.MonadSplit',
-   including `Control.Monad.Random.Class.MonadSplit__StateT__5' *)
-
-(* Skipping all instances of class `Control.Monad.Random.Class.MonadSplit',
-   including `Control.Monad.Random.Class.MonadSplit__ReaderT__5' *)
-
-(* Skipping all instances of class `Control.Monad.Random.Class.MonadSplit',
-   including `Control.Monad.Random.Class.MonadSplit__Strict_RWST__5' *)
-
-(* Skipping all instances of class `Control.Monad.Random.Class.MonadSplit',
-   including `Control.Monad.Random.Class.MonadSplit__RWST__5' *)
-
-(* Skipping all instances of class `Control.Monad.Random.Class.MonadSplit',
-   including `Control.Monad.Random.Class.MonadSplit__MaybeT__5' *)
-
-(* Skipping all instances of class `Control.Monad.Random.Class.MonadSplit',
-   including `Control.Monad.Random.Class.MonadSplit__ListT__5' *)
-
-(* Skipping all instances of class `Control.Monad.Random.Class.MonadSplit',
-   including `Control.Monad.Random.Class.MonadSplit__IdentityT__5' *)
-
-(* Skipping all instances of class `Control.Monad.Random.Class.MonadSplit',
-   including `Control.Monad.Random.Class.MonadSplit__ExceptT__5' *)
-
-(* Skipping all instances of class `Control.Monad.Random.Class.MonadSplit',
-   including `Control.Monad.Random.Class.MonadSplit__ErrorT__5' *)
+   including `Control.Monad.Random.Class.MonadSplit__StdGen__IO' *)
 
 (* Skipping all instances of class `Control.Monad.Random.Class.MonadSplit',
    including `Control.Monad.Random.Class.MonadSplit__ContT__5' *)
 
 (* Skipping all instances of class `Control.Monad.Random.Class.MonadSplit',
-   including `Control.Monad.Random.Class.MonadSplit__StdGen__IO' *)
+   including `Control.Monad.Random.Class.MonadSplit__ErrorT__5' *)
+
+(* Skipping all instances of class `Control.Monad.Random.Class.MonadSplit',
+   including `Control.Monad.Random.Class.MonadSplit__ExceptT__5' *)
+
+(* Skipping all instances of class `Control.Monad.Random.Class.MonadSplit',
+   including `Control.Monad.Random.Class.MonadSplit__IdentityT__5' *)
+
+(* Skipping all instances of class `Control.Monad.Random.Class.MonadSplit',
+   including `Control.Monad.Random.Class.MonadSplit__ListT__5' *)
+
+(* Skipping all instances of class `Control.Monad.Random.Class.MonadSplit',
+   including `Control.Monad.Random.Class.MonadSplit__MaybeT__5' *)
+
+(* Skipping all instances of class `Control.Monad.Random.Class.MonadSplit',
+   including `Control.Monad.Random.Class.MonadSplit__RWST__5' *)
+
+(* Skipping all instances of class `Control.Monad.Random.Class.MonadSplit',
+   including `Control.Monad.Random.Class.MonadSplit__Strict_RWST__5' *)
+
+(* Skipping all instances of class `Control.Monad.Random.Class.MonadSplit',
+   including `Control.Monad.Random.Class.MonadSplit__ReaderT__5' *)
+
+(* Skipping all instances of class `Control.Monad.Random.Class.MonadSplit',
+   including `Control.Monad.Random.Class.MonadSplit__StateT__5' *)
+
+(* Skipping all instances of class `Control.Monad.Random.Class.MonadSplit',
+   including `Control.Monad.Random.Class.MonadSplit__Strict_StateT__5' *)
+
+(* Skipping all instances of class `Control.Monad.Random.Class.MonadSplit',
+   including `Control.Monad.Random.Class.MonadSplit__WriterT__5' *)
+
+(* Skipping all instances of class `Control.Monad.Random.Class.MonadSplit',
+   including `Control.Monad.Random.Class.MonadSplit__Strict_WriterT__5' *)
+
+Local Definition MonadInterleave__ContT_interleave {inst_m : Type -> Type}
+  {inst_r : Type} `{(MonadInterleave inst_m)}
+   : forall {a : Type},
+     Control.Monad.Trans.Cont.ContT inst_r inst_m a ->
+     Control.Monad.Trans.Cont.ContT inst_r inst_m a :=
+  fun {a : Type} => Control.Monad.Trans.Cont.mapContT interleave.
+
+Program Instance MonadInterleave__ContT {m : Type -> Type} {r : Type}
+  `{(MonadInterleave m)}
+   : MonadInterleave (Control.Monad.Trans.Cont.ContT r m) :=
+  fun _ k__ =>
+    k__ {| interleave__ := fun {a : Type} => MonadInterleave__ContT_interleave |}.
+
+(* Skipping instance `Control.Monad.Random.Class.MonadInterleave__ErrorT' of
+   class `Control.Monad.Random.Class.MonadInterleave' *)
+
+Local Definition MonadInterleave__ExceptT_interleave {inst_m : Type -> Type}
+  {inst_e : Type} `{(MonadInterleave inst_m)}
+   : forall {a : Type},
+     Control.Monad.Trans.Except.ExceptT inst_e inst_m a ->
+     Control.Monad.Trans.Except.ExceptT inst_e inst_m a :=
+  fun {a : Type} => Control.Monad.Trans.Except.mapExceptT interleave.
+
+Program Instance MonadInterleave__ExceptT {m : Type -> Type} {e : Type}
+  `{(MonadInterleave m)}
+   : MonadInterleave (Control.Monad.Trans.Except.ExceptT e m) :=
+  fun _ k__ =>
+    k__ {| interleave__ := fun {a : Type} => MonadInterleave__ExceptT_interleave |}.
+
+Local Definition MonadInterleave__IdentityT_interleave {inst_m : Type -> Type}
+  `{(MonadInterleave inst_m)}
+   : forall {a : Type},
+     Control.Monad.Trans.Identity.IdentityT inst_m a ->
+     Control.Monad.Trans.Identity.IdentityT inst_m a :=
+  fun {a : Type} => Control.Monad.Trans.Identity.mapIdentityT interleave.
+
+Program Instance MonadInterleave__IdentityT {m : Type -> Type}
+  `{(MonadInterleave m)}
+   : MonadInterleave (Control.Monad.Trans.Identity.IdentityT m) :=
+  fun _ k__ =>
+    k__ {| interleave__ := fun {a : Type} =>
+             MonadInterleave__IdentityT_interleave |}.
+
+(* Skipping instance `Control.Monad.Random.Class.MonadInterleave__ListT' of
+   class `Control.Monad.Random.Class.MonadInterleave' *)
+
+Local Definition MonadInterleave__MaybeT_interleave {inst_m : Type -> Type}
+  `{(MonadInterleave inst_m)}
+   : forall {a : Type},
+     Control.Monad.Trans.Maybe.MaybeT inst_m a ->
+     Control.Monad.Trans.Maybe.MaybeT inst_m a :=
+  fun {a : Type} => Control.Monad.Trans.Maybe.mapMaybeT interleave.
+
+Program Instance MonadInterleave__MaybeT {m : Type -> Type} `{(MonadInterleave
+   m)}
+   : MonadInterleave (Control.Monad.Trans.Maybe.MaybeT m) :=
+  fun _ k__ =>
+    k__ {| interleave__ := fun {a : Type} => MonadInterleave__MaybeT_interleave |}.
+
+Local Definition MonadInterleave__RWST_interleave {inst_w : Type} {inst_m
+   : Type -> Type} {inst_r : Type} {inst_s : Type} `{GHC.Base.Monoid inst_w}
+  `{MonadInterleave inst_m}
+   : forall {a : Type},
+     Control.Monad.Trans.RWS.Lazy.RWST inst_r inst_w inst_s inst_m a ->
+     Control.Monad.Trans.RWS.Lazy.RWST inst_r inst_w inst_s inst_m a :=
+  fun {a : Type} => Control.Monad.Trans.RWS.Lazy.mapRWST interleave.
+
+Program Instance MonadInterleave__RWST {w : Type} {m : Type -> Type} {r : Type}
+  {s : Type} `{GHC.Base.Monoid w} `{MonadInterleave m}
+   : MonadInterleave (Control.Monad.Trans.RWS.Lazy.RWST r w s m) :=
+  fun _ k__ =>
+    k__ {| interleave__ := fun {a : Type} => MonadInterleave__RWST_interleave |}.
+
+(* Skipping instance `Control.Monad.Random.Class.MonadInterleave__Strict_RWST'
+   of class `Control.Monad.Random.Class.MonadInterleave' *)
+
+Local Definition MonadInterleave__ReaderT_interleave {inst_m : Type -> Type}
+  {inst_r : Type} `{(MonadInterleave inst_m)}
+   : forall {a : Type},
+     Control.Monad.Trans.Reader.ReaderT inst_r inst_m a ->
+     Control.Monad.Trans.Reader.ReaderT inst_r inst_m a :=
+  fun {a : Type} => Control.Monad.Trans.Reader.mapReaderT interleave.
+
+Program Instance MonadInterleave__ReaderT {m : Type -> Type} {r : Type}
+  `{(MonadInterleave m)}
+   : MonadInterleave (Control.Monad.Trans.Reader.ReaderT r m) :=
+  fun _ k__ =>
+    k__ {| interleave__ := fun {a : Type} => MonadInterleave__ReaderT_interleave |}.
+
+Local Definition MonadInterleave__StateT_interleave {inst_m : Type -> Type}
+  {inst_s : Type} `{(MonadInterleave inst_m)}
+   : forall {a : Type},
+     Control.Monad.Trans.State.Lazy.StateT inst_s inst_m a ->
+     Control.Monad.Trans.State.Lazy.StateT inst_s inst_m a :=
+  fun {a : Type} => Control.Monad.Trans.State.Lazy.mapStateT interleave.
+
+Program Instance MonadInterleave__StateT {m : Type -> Type} {s : Type}
+  `{(MonadInterleave m)}
+   : MonadInterleave (Control.Monad.Trans.State.Lazy.StateT s m) :=
+  fun _ k__ =>
+    k__ {| interleave__ := fun {a : Type} => MonadInterleave__StateT_interleave |}.
+
+(* Skipping instance `Control.Monad.Random.Class.MonadInterleave__Strict_StateT'
+   of class `Control.Monad.Random.Class.MonadInterleave' *)
+
+Local Definition MonadInterleave__WriterT_interleave {inst_w : Type} {inst_m
+   : Type -> Type} `{GHC.Base.Monoid inst_w} `{MonadInterleave inst_m}
+   : forall {a : Type},
+     Control.Monad.Trans.Writer.Lazy.WriterT inst_w inst_m a ->
+     Control.Monad.Trans.Writer.Lazy.WriterT inst_w inst_m a :=
+  fun {a : Type} => Control.Monad.Trans.Writer.Lazy.mapWriterT interleave.
+
+Program Instance MonadInterleave__WriterT {w : Type} {m : Type -> Type}
+  `{GHC.Base.Monoid w} `{MonadInterleave m}
+   : MonadInterleave (Control.Monad.Trans.Writer.Lazy.WriterT w m) :=
+  fun _ k__ =>
+    k__ {| interleave__ := fun {a : Type} => MonadInterleave__WriterT_interleave |}.
 
 (* Skipping instance
    `Control.Monad.Random.Class.MonadInterleave__Strict_WriterT' of class
    `Control.Monad.Random.Class.MonadInterleave' *)
 
-Local Definition MonadInterleave__WriterT_interleave {inst_w} {inst_m}
-  `{GHC.Base.Monoid inst_w} `{MonadInterleave inst_m}
-   : forall {a},
-     (Control.Monad.Trans.Writer.Lazy.WriterT inst_w inst_m) a ->
-     (Control.Monad.Trans.Writer.Lazy.WriterT inst_w inst_m) a :=
-  fun {a} => Control.Monad.Trans.Writer.Lazy.mapWriterT interleave.
+(* Skipping definition `Control.Monad.Random.Class.weighted' *)
 
-Program Instance MonadInterleave__WriterT {w} {m} `{GHC.Base.Monoid w}
-  `{MonadInterleave m}
-   : MonadInterleave (Control.Monad.Trans.Writer.Lazy.WriterT w m) :=
-  fun _ k__ =>
-    k__ {| interleave__ := fun {a} => MonadInterleave__WriterT_interleave |}.
+(* Skipping definition `Control.Monad.Random.Class.weightedMay' *)
 
-(* Skipping instance `Control.Monad.Random.Class.MonadInterleave__Strict_StateT'
-   of class `Control.Monad.Random.Class.MonadInterleave' *)
+(* Skipping definition `Control.Monad.Random.Class.fromList' *)
 
-Local Definition MonadInterleave__StateT_interleave {inst_m} {inst_s}
-  `{(MonadInterleave inst_m)}
-   : forall {a},
-     (Control.Monad.Trans.State.Lazy.StateT inst_s inst_m) a ->
-     (Control.Monad.Trans.State.Lazy.StateT inst_s inst_m) a :=
-  fun {a} => Control.Monad.Trans.State.Lazy.mapStateT interleave.
+(* Skipping definition `Control.Monad.Random.Class.fromListMay' *)
 
-Program Instance MonadInterleave__StateT {m} {s} `{(MonadInterleave m)}
-   : MonadInterleave (Control.Monad.Trans.State.Lazy.StateT s m) :=
-  fun _ k__ =>
-    k__ {| interleave__ := fun {a} => MonadInterleave__StateT_interleave |}.
+(* Skipping definition `Control.Monad.Random.Class.uniform' *)
 
-Local Definition MonadInterleave__ReaderT_interleave {inst_m} {inst_r}
-  `{(MonadInterleave inst_m)}
-   : forall {a},
-     (Control.Monad.Trans.Reader.ReaderT inst_r inst_m) a ->
-     (Control.Monad.Trans.Reader.ReaderT inst_r inst_m) a :=
-  fun {a} => Control.Monad.Trans.Reader.mapReaderT interleave.
-
-Program Instance MonadInterleave__ReaderT {m} {r} `{(MonadInterleave m)}
-   : MonadInterleave (Control.Monad.Trans.Reader.ReaderT r m) :=
-  fun _ k__ =>
-    k__ {| interleave__ := fun {a} => MonadInterleave__ReaderT_interleave |}.
-
-(* Skipping instance `Control.Monad.Random.Class.MonadInterleave__Strict_RWST'
-   of class `Control.Monad.Random.Class.MonadInterleave' *)
-
-Local Definition MonadInterleave__RWST_interleave {inst_w} {inst_m} {inst_r}
-  {inst_s} `{GHC.Base.Monoid inst_w} `{MonadInterleave inst_m}
-   : forall {a},
-     (Control.Monad.Trans.RWS.Lazy.RWST inst_r inst_w inst_s inst_m) a ->
-     (Control.Monad.Trans.RWS.Lazy.RWST inst_r inst_w inst_s inst_m) a :=
-  fun {a} => Control.Monad.Trans.RWS.Lazy.mapRWST interleave.
-
-Program Instance MonadInterleave__RWST {w} {m} {r} {s} `{GHC.Base.Monoid w}
-  `{MonadInterleave m}
-   : MonadInterleave (Control.Monad.Trans.RWS.Lazy.RWST r w s m) :=
-  fun _ k__ =>
-    k__ {| interleave__ := fun {a} => MonadInterleave__RWST_interleave |}.
-
-Local Definition MonadInterleave__MaybeT_interleave {inst_m} `{(MonadInterleave
-   inst_m)}
-   : forall {a},
-     (Control.Monad.Trans.Maybe.MaybeT inst_m) a ->
-     (Control.Monad.Trans.Maybe.MaybeT inst_m) a :=
-  fun {a} => Control.Monad.Trans.Maybe.mapMaybeT interleave.
-
-Program Instance MonadInterleave__MaybeT {m} `{(MonadInterleave m)}
-   : MonadInterleave (Control.Monad.Trans.Maybe.MaybeT m) :=
-  fun _ k__ =>
-    k__ {| interleave__ := fun {a} => MonadInterleave__MaybeT_interleave |}.
-
-(* Skipping instance `Control.Monad.Random.Class.MonadInterleave__ListT' of
-   class `Control.Monad.Random.Class.MonadInterleave' *)
-
-Local Definition MonadInterleave__IdentityT_interleave {inst_m}
-  `{(MonadInterleave inst_m)}
-   : forall {a},
-     (Control.Monad.Trans.Identity.IdentityT inst_m) a ->
-     (Control.Monad.Trans.Identity.IdentityT inst_m) a :=
-  fun {a} => Control.Monad.Trans.Identity.mapIdentityT interleave.
-
-Program Instance MonadInterleave__IdentityT {m} `{(MonadInterleave m)}
-   : MonadInterleave (Control.Monad.Trans.Identity.IdentityT m) :=
-  fun _ k__ =>
-    k__ {| interleave__ := fun {a} => MonadInterleave__IdentityT_interleave |}.
-
-Local Definition MonadInterleave__ExceptT_interleave {inst_m} {inst_e}
-  `{(MonadInterleave inst_m)}
-   : forall {a},
-     (Control.Monad.Trans.Except.ExceptT inst_e inst_m) a ->
-     (Control.Monad.Trans.Except.ExceptT inst_e inst_m) a :=
-  fun {a} => Control.Monad.Trans.Except.mapExceptT interleave.
-
-Program Instance MonadInterleave__ExceptT {m} {e} `{(MonadInterleave m)}
-   : MonadInterleave (Control.Monad.Trans.Except.ExceptT e m) :=
-  fun _ k__ =>
-    k__ {| interleave__ := fun {a} => MonadInterleave__ExceptT_interleave |}.
-
-(* Skipping instance `Control.Monad.Random.Class.MonadInterleave__ErrorT' of
-   class `Control.Monad.Random.Class.MonadInterleave' *)
-
-Local Definition MonadInterleave__ContT_interleave {inst_m} {inst_r}
-  `{(MonadInterleave inst_m)}
-   : forall {a},
-     (Control.Monad.Trans.Cont.ContT inst_r inst_m) a ->
-     (Control.Monad.Trans.Cont.ContT inst_r inst_m) a :=
-  fun {a} => Control.Monad.Trans.Cont.mapContT interleave.
-
-Program Instance MonadInterleave__ContT {m} {r} `{(MonadInterleave m)}
-   : MonadInterleave (Control.Monad.Trans.Cont.ContT r m) :=
-  fun _ k__ =>
-    k__ {| interleave__ := fun {a} => MonadInterleave__ContT_interleave |}.
+(* Skipping definition `Control.Monad.Random.Class.uniformMay' *)
 
 (* External variables:
      Type list op_zt__ Control.Monad.Trans.Class.lift Control.Monad.Trans.Cont.ContT
