examples/shuffle/lib/Data/List/Shuffle.v
@@ -63,29 +63,30 @@ Import GHC.Num.Notations.
 
 (* Converted value declarations: *)
 
-Program Fixpoint riffle {m} {a} `{Control.Monad.Random.Class.MonadRandom m}
-                        (arg_0__ : list a) (arg_1__ : GHC.Num.Int) (arg_2__ : list a) (arg_3__
-                          : GHC.Num.Int) {measure (length arg_0__ + length arg_2__)} : m (list a)
-                   := match arg_0__, arg_1__, arg_2__, arg_3__ with
-                      | xs, _, nil, _ => GHC.Base.pure xs
-                      | nil, _, ys, _ => GHC.Base.pure ys
-                      | cons x xs, nx, cons y ys, ny =>
-                          Control.Monad.Random.Class.getRandomR (pair #1 (nx GHC.Num.+ ny)) GHC.Base.>>=
-                          (fun k =>
-                             if Bool.Sumbool.sumbool_of_bool (k GHC.Base.<= nx)
-                             then (fun arg_6__ => cons x arg_6__) Data.Functor.<$>
-                                  riffle xs (nx GHC.Num.- #1) (cons y ys) ny
-                             else (fun arg_7__ => cons y arg_7__) Data.Functor.<$>
-                                  riffle (cons x xs) nx ys (ny GHC.Num.- #1))
-                      end.
-Solve Obligations with (solve_riffle).
+Fixpoint halve {a : Type} (arg_0__ : list a) : (list a * list a)%type
+  := match arg_0__ with
+     | nil => pair nil nil
+     | cons z zs => let 'pair xs ys := halve zs in pair (cons z ys) xs
+     end.
 
-Definition halve {a} : list a -> (list a * list a)%type :=
-  fix halve arg_0__
-        := match arg_0__ with
-           | nil => pair nil nil
-           | cons z zs => let 'pair xs ys := halve zs in pair (cons z ys) xs
-           end.
+Program Fixpoint riffle {m : Type -> Type} {a : Type}
+                        `{Control.Monad.Random.Class.MonadRandom m} (arg_0__ : list a) (arg_1__
+                          : GHC.Num.Int) (arg_2__ : list a) (arg_3__ : GHC.Num.Int) {measure (length
+                         arg_0__ +
+                         length arg_2__)} : m (list a)
+  := match arg_0__, arg_1__, arg_2__, arg_3__ with
+     | xs, _, nil, _ => GHC.Base.pure xs
+     | nil, _, ys, _ => GHC.Base.pure ys
+     | cons x xs, nx, cons y ys, ny =>
+         Control.Monad.Random.Class.getRandomR (pair #1 (nx GHC.Num.+ ny)) GHC.Base.>>=
+         (fun k =>
+            if Bool.Sumbool.sumbool_of_bool (k GHC.Base.<= nx)
+            then (fun arg_6__ => cons x arg_6__) Data.Functor.<$>
+                 riffle xs (nx GHC.Num.- #1) (cons y ys) ny
+            else (fun arg_7__ => cons y arg_7__) Data.Functor.<$>
+                 riffle (cons x xs) nx ys (ny GHC.Num.- #1))
+     end.
+Solve Obligations with (solve_riffle).
 
 Theorem length_halve {a} (zs : list a) : let 'pair xs ys := halve zs in
   length xs = Nat.div2 (S (length zs)) /\ length ys = Nat.div2 (length zs).
@@ -98,31 +99,33 @@ Proof.
   - now rewrite IHxs; simpl.
 Qed.
 
-Program Fixpoint shuffleLength {m} {a} `{Control.Monad.Random.Class.MonadRandom
-                               m} (arg_0__ : list a) {measure (length arg_0__)} : m (list a * GHC.Num.Int)%type
-                   := match arg_0__ with
-                      | nil => GHC.Base.pure (pair nil #0)
-                      | cons x nil => GHC.Base.pure (pair (cons x nil) #1)
-                      | xs =>
-                          let 'pair half1 half2 := halve xs in
-                          let cont_4__ arg_5__ :=
-                            let 'pair shuffled1 length1 := arg_5__ in
-                            let cont_6__ arg_7__ :=
-                              let 'pair shuffled2 length2 := arg_7__ in
-                              riffle shuffled1 length1 shuffled2 length2 GHC.Base.>>=
-                              (fun shuffled => GHC.Base.pure (pair shuffled (length1 GHC.Num.+ length2))) in
-                            shuffleLength half2 GHC.Base.>>= cont_6__ in
-                          shuffleLength half1 GHC.Base.>>= cont_4__
-                      end.
+Program Fixpoint shuffleLength {m : Type -> Type} {a : Type}
+                               `{Control.Monad.Random.Class.MonadRandom m} (arg_0__ : list a) {measure (length
+                                arg_0__)} : m (list a * GHC.Num.Int)%type
+  := match arg_0__ with
+     | nil => GHC.Base.pure (pair nil #0)
+     | cons x nil => GHC.Base.pure (pair (cons x nil) #1)
+     | xs =>
+         let 'pair half1 half2 := halve xs in
+         let cont_4__ arg_5__ :=
+           let 'pair shuffled1 length1 := arg_5__ in
+           let cont_6__ arg_7__ :=
+             let 'pair shuffled2 length2 := arg_7__ in
+             riffle shuffled1 length1 shuffled2 length2 GHC.Base.>>=
+             (fun shuffled => GHC.Base.pure (pair shuffled (length1 GHC.Num.+ length2))) in
+           shuffleLength half2 GHC.Base.>>= cont_6__ in
+         shuffleLength half1 GHC.Base.>>= cont_4__
+     end.
 Solve Obligations with (solve_shuffleLength @halve @length_halve).
 
-Definition shuffle {m} {a} `{Control.Monad.Random.Class.MonadRandom m}
+Definition shuffle {m : Type -> Type} {a : Type}
+  `{Control.Monad.Random.Class.MonadRandom m}
    : list a -> m (list a) :=
   GHC.Base.fmap Data.Tuple.fst GHC.Base.∘ shuffleLength.
 
 (* External variables:
-     Bool.Sumbool.sumbool_of_bool S cons length list nil op_ze__ op_zp__ op_zszr__
-     op_zt__ pair Control.Monad.Random.Class.MonadRandom
+     Bool.Sumbool.sumbool_of_bool S Type cons length list nil op_ze__ op_zp__
+     op_zszr__ op_zt__ pair Control.Monad.Random.Class.MonadRandom
      Control.Monad.Random.Class.getRandomR Data.Functor.op_zlzdzg__ Data.Tuple.fst
      GHC.Base.fmap GHC.Base.op_z2218U__ GHC.Base.op_zgzgze__ GHC.Base.op_zlze__
      GHC.Base.pure GHC.Num.Int GHC.Num.fromInteger GHC.Num.op_zm__ GHC.Num.op_zp__
